Trying to simplify simulation on call ev

theories/vir/contextual/contextual.v
@@ -108,12 +108,12 @@ Section CR_definition.
   (* Filling the context involves (1) extending the function declaration map and
     (2) restating the denotation of mutually-recursive control flow graps using
         [denote_mcfg]. *)
-  Definition fill_ctx (C : context) e :=
+  Definition fill_ctx (C : context) e attr :=
     Monad.bind (mcfg_definitions (fill_mcfg_defs C e))
-        (fun defs => denote_mcfg defs ret_typ (DVALUE_Addr main) args).
+        (fun defs => denote_mcfg defs ret_typ (DVALUE_Addr main) args attr).
 
   (* Contextual refinement. *)
-  Definition ctx_ref e_t e_s: Prop :=
+  Definition ctx_ref e_t e_s attr: Prop :=
     forall (C : CFG.mcfg dtyp),
       (* The context and function needs to be well-formed *)
       ctx_wf C ->
@@ -121,7 +121,7 @@ Section CR_definition.
       (* All the attributes are nil *)
       (Forall (fun x => dc_attrs x = nil) (map df_prototype (m_definitions C))) ->
       (* Implies whole-program refinement *)
-      prog_ref (m_declarations C) main (fill_ctx C e_t) (fill_ctx C e_s).
+      prog_ref (m_declarations C) main (fill_ctx C e_t attr) (fill_ctx C e_s attr).
 
 End CR_definition.
 
@@ -133,17 +133,12 @@ Section contextual_refinement.
 
   Definition mcfg_logrel
     (Ft Fs : list (dvalue * definition dtyp (cfg dtyp)))
-    τ ft fs (args_t args_s : list uvalue) : iPropI Σ :=
-    (∀ i_t i_s args_t args_s,
-      frameR i_t i_s nil nil ∅ -∗
-      allocaR i_t i_s ∅ ∅ -∗
-      val_rel.Forall2 uval_rel args_t args_s -∗
-      denote_mcfg Ft τ ft args_t ⪯
-      denote_mcfg Fs τ fs args_s
+    τ ft fs (args_t args_s : list uvalue) attr : iPropI Σ :=
+    (val_rel.Forall2 uval_rel args_t args_s -∗
+      denote_mcfg Ft τ ft args_t attr ⪯
+      denote_mcfg Fs τ fs args_s attr
     ⦉ fun v_t v_s =>
         ∃ r_t r_s, ⌜v_t = Ret r_t⌝ ∗ ⌜v_s = Ret r_s⌝ ∗
-        frameR i_t i_s nil nil ∅∗
-        allocaR i_t i_s ∅ ∅ ∗
         uval_rel r_t r_s ⦊)%I.
 
   Definition interp_mrec_body {D E : Type -> Type}
@@ -156,27 +151,213 @@ Section contextual_refinement.
       | @VisF _ _ _ X (inr1 e) k => Vis e (λ x0 : X, Ret (inl (k x0)))
       end.
 
-  Opaque denote_function.
-  Lemma denote_mcfg_unfold l τ (f : dvalue) args x:
-    lookup_defn f l = Some x ->
-    RelDec.rel_dec (dc_attrs (df_prototype x)) (remove_tag []) ->
-    denote_mcfg l τ f args ≅
-      lr <- interp_mrec_body (denote_mfun l) _ (denote_function x args) ;;
-      match lr with
-      | inl l0 => Tau (interp_mrec (denote_mfun l) l0)
-      | inr r => Ret r
-      end.
-  Proof.
-    intros H Hattr; rewrite /denote_mcfg.
-    rewrite {1}/mrec /interp_mrec.
-    setoid_rewrite unfold_iter at 1.
-    change (ITree.iter _) with (interp_mrec (T := uvalue) (denote_mfun l)).
-    rewrite {1}/denote_mfun. rewrite H.
-    fold (interp_mrec (D := CallE) (E := L0)); rewrite Hattr.
-    eapply eq_itree_clo_bind; first done. intros; subst; done.
-  Qed.
+  Definition lift_val_rel {R1 R2} (Φ : R1 -> R2 -> iPropI Σ) :=
+    (λ (x : exprO (Λ := vir_lang) R1) (y : exprO (Λ := vir_lang) R2),
+        ∃ vx vy, ⌜x = Ret vx⌝ ∗ ⌜y = Ret vy⌝ ∗ Φ vx vy)%I.
+
+  Definition interp_mrec_post (Φ : uvalue -> uvalue -> iPropI Σ) :=
+    (fun vx vy =>
+      match vx, vy with
+      | inl x, inl y => L0'expr_conv x ⪯ L0'expr_conv y [{ (x, y), Φ x y }]
+      | inr x, inr y => Φ x y | _, _ => ⌜False⌝
+      end)%I.
 
   From Paco Require Import paco.
+
+  Lemma interp_mrec_body_proper {D E} x y ctx ctx':
+    x ≅ y ->
+    (∀ u d, ctx u d ≅ ctx' u d) ->
+    eq_itree (fun x y => match x, y with
+      | inl x, inl y => x ≅ y | inr x, inr y => x = y | _, _ => False end)
+      (interp_mrec_body ctx uvalue x)
+      (interp_mrec_body (D := D) (E := E) ctx' uvalue y).
+  Proof.
+    intros Heq Hctx. punfold Heq. red in Heq.
+    unfold interp_mrec_body.
+    remember (observe x) as Hox; remember (observe y) as Hoy.
+    clear HeqHox HeqHoy.
+    destruct Heq; subst; try done; pclearbot; try apply eqit_Ret; try done.
+    destruct e; try apply eqit_Ret.
+    - eapply eq_itree_clo_bind; first done; intros; subst; eauto.
+      eapply REL.
+    - apply eqit_Vis; intros. apply eqit_Ret; apply REL.
+  Qed.
+
+  Notation "x ~d~ y" := (dval_rel x y) (at level 20).
+  Notation "x ~u~ y" := (uval_rel x y) (at level 20).
+  Notation "x ~U~ y" := (val_rel.Forall2 uval_rel x y) (at level 20).
+
+  (* Lemma sim_expr'_ret_inv {R1 R2} r_t r_s (Φ : R1 -> R2 -> iPropI Σ) : *)
+  (*   Ret r_t ⪯ Ret r_s ⦉ lift_val_rel Φ ⦊ -∗ *)
+  (*   Φ r_t r_s. *)
+  (* Proof. *)
+  (*   rewrite sim_expr' _unfold. *)
+  (*   iIntros "[SI H]". rewrite sim_expr_unfold. cbn. *)
+  (*   iSpecialize ("H" with "SI"). iMod "H". iDestruct "H" as (?) "H". *)
+  (*   destruct c. *)
+  (*   - rewrite /lift_expr_rel. *)
+  (*     iDestruct "H" as (??????) "(?&H)". *)
+  (*     iDestruct "H" as (????) "H". *)
+  (*     apply eqit_inv in H; apply eqit_inv in H0. *)
+  (*     cbn in H, H0. inv H; inv H0. *)
+  (*     subst. *)
+  (*     apply eqit_inv in H1; apply eqit_inv in H2. *)
+  (*     cbn in H1, H2. subst. *)
+  (*     iModIntro; iFrame. *)
+  (*   - rewrite /stutter_l. *)
+  (*     iDestruct "H" as (??) "H". inv H. *)
+  (*   - rewrite /stutter_r. *)
+  (*     iDestruct "H" as (??) "H". inv H. *)
+  (*   - rewrite /tau_step. *)
+  (*     iDestruct "H" as (???) "H". inv H. *)
+  (*   - rewrite /vis_step. *)
+  (*     iDestruct "H" as (???????) "H". inv H. *)
+  (*   - rewrite /source_ub. *)
+  (*     iDestruct "H" as (???) "%H". inv H. *)
+  (*   - rewrite /source_exc. *)
+  (*     iDestruct "H" as (???) "%H". inv H. *)
+  (* Qed. *)
+
+  Lemma sim_coindF_ret_inv {R1 R2} r1 r2 (Φ: R1 -d> R2 -d> iPropI Σ) :
+    ⊢ sim_coindF (lift_rel (lift_val_rel Φ)) (RetF r1) (RetF r2) ==∗
+      state_interp r1.1 r2.1 ∗ Φ r1.2 r2.2.
+  Proof.
+    iIntros "H".
+    rewrite sim_coindF_unfold sim_indF_unfold /sim_expr_inner. iMod "H".
+    iDestruct "H" as (?) "H".
+    destruct c.
+    - rewrite /lift_rel /lift_val_rel.
+      iDestruct "H" as (????)"(SI & H)".
+      iDestruct "H" as (??????) "H"; subst.
+      cbn -[state_interp] in *. inv H; inv H0. by iFrame.
+    - rewrite /stutter_l.
+      iDestruct "H" as (??) "H". inv H.
+    - rewrite /stutter_r.
+      iDestruct "H" as (??) "H". inv H.
+    - rewrite /tau_step.
+      iDestruct "H" as (???) "H". inv H.
+    - rewrite /vis_step.
+      iDestruct "H" as (????????) "H". inv H0.
+    - rewrite /source_ub.
+      iDestruct "H" as (???) "%H". inv H.
+    - rewrite /source_exc.
+      iDestruct "H" as (???) "%H". inv H.
+  Qed.
+
+  Lemma interp_mrec_body_proper' (x : itree L0' uvalue) (y : itree L0' uvalue)
+    (ctx ctx' : ∀ T : Type, CallE T → L0'expr T) Φ :
+    ⟅ x ⟆ ⪯ ⟅ y ⟆ ⦉ lift_val_rel Φ ⦊ -∗
+    (∀ τ f_t f_s attrs args_t args_s,
+        f_t ~d~ f_s -∗
+        args_t ~U~ args_s -∗
+        ⟅ ctx _ (Call τ f_t args_t attrs) ⟆ ⪯
+        ⟅ ctx' _ (Call τ f_s args_s attrs) ⟆
+        ⦉ lift_val_rel uval_rel ⦊) -∗
+    interp_mrec_body (D := CallE) ctx uvalue x
+    ⪯
+    interp_mrec_body (D := CallE) ctx' uvalue y
+    ⦉ lift_val_rel (interp_mrec_post Φ) ⦊.
+  Proof.
+    iIntros "H Hctx".
+    rewrite /interp_mrec_body.
+    rewrite {1 2}/L0'expr_conv; do 2 rewrite unfold_interp.
+
+    destruct (observe x) eqn: Hx; destruct (observe y) eqn: Hy; rewrite Hx Hy; cbn.
+    { (* Ret Ret *)
+      iIntros (??) "SI".
+      iSpecialize ("H" with "SI"). iMod "H".
+      rewrite /interp_L2. setoid_rewrite StateFacts.interp_state_ret.
+      rewrite /sim_coind'. cbn.
+      iMod (sim_coindF_ret_inv with "H") as "(SI & H)".
+      iApply sim_coindF_base; cbn.
+      iExists σ_t, σ_s, (Ret (inr r)), (Ret (inr r0)).
+      sfinal. cbn; do 2 sfinal. }
+    8 : {
+      destruct e, e0; eauto.
+      { iApply sim_expr'_base. sfinal. rewrite /interp_mrec_post.
+        destruct c, c0. rewrite !bind_vis.
+        iPoseProof (sim_expr'_call_inv with "H") as "H".
+  Admitted.
+
+  Lemma denote_mfun_related args_t args_s attr ft fs τ F_t F_s :
+    val_rel.Forall2 uval_rel args_t args_s -∗
+    ⟅ denote_mfun F_t (Call τ ft args_t attr) ⟆
+    ⪯
+    ⟅ denote_mfun F_s (Call τ fs args_s attr) ⟆
+    ⦉ lift_val_rel uval_rel ⦊.
+  Proof. Admitted.
+
+  Lemma base_rel_eq:
+    ⊢ □
+      (∀ x y,
+        sim_properties.base (Λ := vir_lang) x y ∗ lift_val_rel uval_rel x y ∗-∗
+        lift_val_rel uval_rel x y).
+  Proof. Admitted.
+
+  (** *contextual refinement *)
+  Theorem contextual_refinement attr C f args τ F:
+    <pers> ([∗ list]
+       '(ft, e_t);'(fs, e_s) ∈ F; F,
+        (* Function names are the same and *)
+        ⌜ft = fs⌝ ∗
+        ⌜dc_attrs (df_prototype e_t) = dc_attrs (df_prototype e_s)⌝ ∗
+        (* The functions are logically related and satisfy the attributes *)
+        fun_logrel attr_inv (dc_attrs (df_prototype e_t)) e_t e_s C) -∗
+    mcfg_logrel F F τ f f args args attr.
+  Proof with vsimp.
+    iIntros "#Hf Hargs"; rewrite /mrec /interp_mrec.
+
+    (* Can change the current subgoal to a guarded iteration*)
+    iApply sim_expr'_tau_inv; first iApply base_rel_eq.
+
+    iApply (sim_expr_guarded_iter'%I).
+    Unshelve.
+    3 : exact
+      (fun x y => sim_expr' (lift_val_rel uval_rel)%I
+                 (L0'expr_conv x) (L0'expr_conv y)).
+    { iModIntro; iIntros (??) "H".
+      iApply sim_expr'_bupd_mono; cycle 1.
+      { iApply (interp_mrec_body_proper' _ _ (denote_mfun F_t) with "[H]");
+          try done;
+        iIntros (??????) "Hdv Hrel".
+        by iApply denote_mfun_related. }
+
+      iIntros (??) "H"; iDestruct "H" as (????) "H"; subst...
+      destruct vx, vy; eauto.
+      { iLeft. sfinal. iApply sim_expr_lift.
+        mono: iApply "H"... cbn. iIntros (??) "H".
+        iDestruct "H" as (????) "H".
+        sfinal. iPureIntro; split; by apply EqAxiom.bisimulation_is_eq. }
+      { iRight. do 2 sfinal. } }
+
+    cbn -[denote_mfun]. by iApply denote_mfun_related.
+  Qed.
+
+End contextual_refinement.
+
+
+  (* Opaque denote_function. *)
+  (* Lemma denote_mcfg_unfold l τ (f : dvalue) args x attr: *)
+  (*   lookup_defn f l = Some x -> *)
+  (*   RelDec.rel_dec (dc_attrs (df_prototype x)) (remove_tag []) -> *)
+  (*   denote_mcfg l τ f args attr ≅ *)
+  (*     lr <- interp_mrec_body (denote_mfun l) _ (denote_function x args) ;; *)
+  (*     match lr with *)
+  (*     | inl l0 => Tau (interp_mrec (denote_mfun l) l0) *)
+  (*     | inr r => Ret r *)
+  (*     end. *)
+  (* Proof. *)
+  (*   intros H Hattr; rewrite /denote_mcfg. *)
+  (*   rewrite {1}/mrec /interp_mrec. *)
+  (*   setoid_rewrite unfold_iter at 1. *)
+  (*   change (ITree.iter _) with (interp_mrec (T := uvalue) (denote_mfun l)). *)
+  (*   rewrite {1}/denote_mfun. rewrite H. *)
+
+  (* (*   fold (interp_mrec (D := CallE) (E := L0)); rewrite Hattr. *) *)
+  (* (*   eapply eq_itree_clo_bind; first done. intros; subst; done. *) *)
+  (* (* Qed. *) *)
+  (* Admitted. *)
+
 
   Lemma interp_mrec_body_proper {D E} x y ctx ctx':
     x ≅ y ->
@@ -196,62 +377,3 @@ Section contextual_refinement.
       eapply REL.
     - apply eqit_Vis; intros. apply eqit_Ret; apply REL.
   Qed.
-
-  Lemma interp_mrec_body_proper' {R} (x : itree L0' R) (y : itree L0' R)
-    (ctx ctx' : ∀ T : Type, CallE T → L0'expr T) Φ :
-    (L0'expr_conv x ⪯ L0'expr_conv y
-       ⦉ fun x y => ∃ vx vy, ⌜x = Ret vx⌝ ∗ ⌜y = Ret vy⌝ ∗  Φ vx vy ⦊) -∗
-    (∀ d, L0'expr_conv (ctx R d) ⪯ L0'expr_conv (ctx' R d)
-         ⦉ fun x y => ∃ vx vy, ⌜x = Ret vx⌝ ∗ ⌜y = Ret vy⌝ ∗  Φ vx vy ⦊) -∗
-    interp_mrec_body (D := CallE) (E := L0) ctx R x
-    ⪯
-    interp_mrec_body (D := CallE) ctx' R y
-    ⦉ fun x y =>
-         ∃ vx vy, ⌜x = Ret vx⌝ ∗ ⌜y = Ret vy⌝ ∗
-          match vx, vy with
-          | inl x, inl y => L0'expr_conv x ⪯ L0'expr_conv y [{ (x, y), Φ x y }]
-          | inr x, inr y => Φ x y | _, _ => ⌜False⌝
-          end ⦊.
-  Proof. Admitted.
-
-  (** *contextual refinement *)
-  Theorem contextual_refinement
-    e_t e_s e_t' e_s' C attr attr' ft ft' fs fs' args_t args_s τ:
-    RelDec.rel_dec (dc_attrs (df_prototype e_t)) [] ->
-    RelDec.rel_dec (dc_attrs (df_prototype e_s)) [] ->
-    fun_logrel attr_inv attr e_t e_s C -∗
-    fun_logrel attr_inv attr' e_t' e_s' C -∗
-    mcfg_logrel
-      [(ft, e_t); (ft', e_t')]
-      [(fs, e_s); (fs', e_s')] τ ft fs args_t args_s.
-  Proof.
-    intros Hat Has.
-    iIntros "Hf Hf'" (????) "Hfr Ha Hargs".
-    rewrite /mrec /interp_mrec.
-    rewrite denote_mcfg_unfold; cycle 1; cbn.
-    { destruct (RelDec.rel_dec ft ft) eqn: Ht; eauto.
-      apply RelDec.neg_rel_dec_correct in Ht; done. }
-    { done. }
-
-    rewrite denote_mcfg_unfold; cycle 1; cbn.
-    { destruct (RelDec.rel_dec fs fs) eqn: Ht; eauto.
-      apply RelDec.neg_rel_dec_correct in Ht; done. }
-    { done. }
-
-    Cut...
-
-    iPoseProof
-      (interp_mrec_body_proper'
-          (denote_function e_t args_t0)
-          (denote_function e_s args_s0)
-          (denote_mfun [(ft, e_t); (ft', e_t')])
-      ) as "H".
-    iApply sim_expr'_bupd_mono; cycle 1.
-    { iApply ("H" with "[Hf Hfr Ha Hargs]").
-      { iApply "Hf"; admit. }
-      iIntros (?). Require Import Coq.Program.Equality.
-      dependent destruction d; cbn.
-
-  Admitted.
-
-End contextual_refinement.
